add pivot branch state machine spec, split proofs into a refinemment file

Splinter/AllocationsLayer/Compactor.i.dfy
@@ -3,7 +3,7 @@
 
 // include "../LikesAU.i.dfy"
 // include "../Journal/MiniAllocator.i.dfy"   // tony: borrowing from Journal for now
-include "../Betree/LinkedBranch.i.dfy"
+include "../Betree/AllocationBranch.i.dfy"
 include "../Betree/BranchSeq.i.dfy"
 include "../Betree/OffsetMap.i.dfy"
 include "MiniAllocator.i.dfy"
@@ -11,7 +11,7 @@ include "LikesAU.i.dfy"
 
 module CompactorMod
 {
-  import opened LinkedBranchMod
+  import opened AllocationBranchMod
   import opened BranchSeqMod
   import opened OffsetMapMod
   import opened MiniAllocatorMod
@@ -19,7 +19,12 @@ module CompactorMod
   import opened GenericDisk
   import opened Sequences
 
-  type BranchDiskView = LinkedBranchMod.DiskView
+  type BranchDiskView = AllocationBranchMod.DiskView
+
+  // label: addresses 
+
+  // 
+
 
 // Transitions for each thread state machine, from the persective of the caller:
   //  Init(compact start), Internal, Commit, Abort
@@ -30,7 +35,13 @@ module CompactorMod
     subdisk: BranchDiskView, // diskview containing exactly the part of the tree we are reading
     // Mutating outputs
     miniAllocator: MiniAllocator,
-    output: LinkedBranch // root of the tree that we are building. Everything reachable from here is mini-allocated, disk here should be consistent with mini-allocator
+
+
+    // all keys to the left of this (exclusive) have been copied to output
+    // 
+    nextKey: Element
+
+    output: AllocationBranch // root of the tree that we are building. Everything reachable from here is mini-allocated, disk here should be consistent with mini-allocator
   ) {
     predicate WF() {
       && miniAllocator.WF()
@@ -55,13 +66,13 @@ module CompactorMod
   datatype TransitionLabel =
     | Begin(branchSeq: BranchSeq, offsetMap: OffsetMap, subdisk: BranchDiskView)
     | Internal(allocs: seq<AU>)
-    | Commit(branchSeq: BranchSeq, offsetMap: OffsetMap, subdisk: BranchDiskView, output: LinkedBranch)
+    | Commit(branchSeq: BranchSeq, offsetMap: OffsetMap, subdisk: BranchDiskView, output: AllocationBranch)
     | Abort(deallocs: seq<AU>)  // allow us to abandon a compaction (even though in practice this is not necessary, via scheduler magic)
 
   datatype Step = 
     | BeginStep()
     | AllocStep(idx: nat)
-    | BuildStep(idx: nat, addr: Address, newOutput: LinkedBranch)
+    | BuildStep(idx: nat, addr: Address, newOutput: AllocationBranch)
     | CommitStep(idx: nat)
     | AbortStep(idx: nat)
 
@@ -74,7 +85,7 @@ module CompactorMod
       lbl.offsetMap, 
       lbl.subdisk, 
       EmptyMiniAllocator(), 
-      LinkedBranch(GenericDisk.Address(0, 0), EmptyDisk())  //placeholder
+      AllocationBranch(GenericDisk.Address(0, 0), EmptyDisk())  //TODO placeholder
       );
     && v' == v.(threads := v.threads + [newThread])
   }
@@ -89,14 +100,34 @@ module CompactorMod
     && v' == v.(threads := v.threads[ idx := thread'])
   }
 
-  predicate Build(v: Variables, v': Variables, lbl: TransitionLabel, idx:nat, addr: Address, newOutput: LinkedBranch) {
+  // move to allocation branch
+  datatype BranchLabel = 
+    | BuildLabel(addrs: seq<Address>, inputStream: FlattenedBranch)
+
+  predicate Build(v: Variables, v': Variables, lbl: TransitionLabel, idx:nat, 
+    addr: Address, newOutput: AllocationBranch, newNextKey: Element) {
     && v.WF()
     && lbl.Internal?
     && idx < |v.threads|
     && lbl.allocs == []
     && var thread := v.threads[idx];
     && thread.miniAllocator.CanAllocate(addr)
+    // nondeterministic transition on the tree
+    // TODO: also take in a tree step so that we can update the tree
+    // new label for updated tree data
+
+    // lbl to branch
+    // lbl: addresses, keys and values to insert
+    // range comparison should be elements
+    && Keys.lte(v.nextKey, newNextKey)
+    && AllocationBranch.Next(v.output, newOutput, 
+      BranchLabel.BuildLabel([addr], branchSeq.toFlattenBranch(v.nextKey, newNextKey)))
+
     && newOutput == thread.output // TODO: This is a placeholder for building the tree
+    // incremental 
+    // several input streams
+    // key consumed based on input streams
+
     && var thread' := thread.(
       miniAllocator := thread.miniAllocator.Allocate(addr),
       output := newOutput 
@@ -112,10 +143,18 @@ module CompactorMod
     && lbl.branchSeq == thread.branchSeq
     && lbl.offsetMap == thread.offsetMap
     && lbl.subdisk == thread.subdisk
-    && true // TODO: placeholder for thread.output is done
-    && lbl.output == thread.output
+
+    && v.nextKey == Element.max // 
+    // representation is the same
+    // && lbl.branchSeq.QueryFilteredEquiv(lbl.subdisk, lbl.offsetMap, lbl.output)
+    // ^ needs an 
+    
+    // && true // TODO: placeholder for thread.output is done
+    // && lbl.output == thread.output
     // reserved set should be same as output.repr, to mean that I used all the stuff I reserved
     && thread.miniAllocator.GetAllReserved() == thread.output.Representation()
     && v'.threads == remove(v.threads, idx)
   }
+
+
 }
