Splinter/Betree/PivotBranch.i.dfy
@@ -24,6 +24,11 @@ module PivotBranchMod {
   import KeysImpl = Lexicographic_Byte_Order_Impl
   import Keys = KeysImpl.Ord
 
+  datatype TransitionLabel = 
+    | QueryLabel(key: Key, msg: Message)
+    | InsertLabel(key: Key, msg: Message)
+    | InternalLabel()
+
   // Flattened branch for iterators (sequential and merge)
   datatype FlattenedBranch = FlattenedBranch(keys: seq<Key>, msgs: seq<Message>)
   {
@@ -94,7 +99,6 @@ module PivotBranchMod {
         && (forall i :: 0 <= i < |children| ==> children[i].WF())
         && (forall i :: 0 <= i < |children|-1 ==> AllKeysBelowBound(i))
         && (forall i :: 0 < i < |children|   ==> AllKeysAboveBound(i))
-        // && (forall i :: 0 <= i < |children| ==> children[i].AllKeys() != {})
     }
 
     function Route(key: Key) : int
@@ -168,7 +172,6 @@ module PivotBranchMod {
       )
     }
 
-    // Note: intended for iterator which we currently don't have
     function Flatten() : (result: FlattenedBranch)
     requires WF()
     ensures result.WF()
@@ -188,6 +191,43 @@ module PivotBranchMod {
       && Flatten() == b
     }
 
+    // We need to measure the height of Nodes to manage termination in the mutual
+    // recursion between InsertNode and InsertIndex. You'd think that we wouldn't
+    // need to, since datatypes are well-founded. But when we SplitChildOfIndex,
+    // we replace some children with other children. The new children are of no
+    // greater height, but they don't order in Dafny's internal datatype lattice.
+    // Hence this machinery for explicitly measuring height.
+    function IndexHeights(): seq<int>
+      requires WF()
+      requires Index?
+      decreases this, 0
+    {
+        seq(|children|, i requires 0<=i<|children| => children[i].Height())
+    }
+
+    function {:opaque} Height(): nat
+      requires WF()
+      ensures Leaf? ==> Height() == 0
+      decreases this, 1
+    {
+      if Leaf?
+      then 0
+      else
+        var heights := IndexHeights(); seqMax(heights) + 1
+    }
+
+    lemma ChildrenAreShorter(childIdx: nat)
+      requires WF()
+      requires Index?
+      requires 0 <= childIdx < |children|
+      ensures children[childIdx].Height() < Height()
+    {
+      var child := children[childIdx];
+      assert IndexHeights()[childIdx] == child.Height(); // trigger
+      assert child.Height() in IndexHeights();  // trigger *harder*
+      reveal_Height();
+    }
+
     // Mutable operations 
 
     // Grow
@@ -196,103 +236,135 @@ module PivotBranchMod {
       Index([], [this])
     }
 
-    lemma GrowPreservesWF()
-      requires WF()
-      requires AllKeys() != {}
-      ensures Grow().WF()
-    {
-      assert Keys.IsStrictlySorted([]) by {
-        Keys.reveal_IsStrictlySorted();
-      }
-    }
-
-    lemma GrowPreservesAllKeys()
-      requires WF()
-      ensures Grow().AllKeys() == AllKeys()
-    {
-      assert forall key :: key in AllKeys() ==> key in Grow().children[0].AllKeys();
-    }
-
-    lemma InterpretationDelegation(key: Key)
-      requires WF()
-      requires Index?
-      requires key in children[Keys.LargestLte(pivots, key)+1].I().mapp
-      ensures MapsTo(I().mapp, key, children[Keys.LargestLte(pivots, key)+1].I().mapp[key])
-    {
-      var interp := I().mapp;
-      assert key in children[Keys.LargestLte(pivots, key)+1].AllKeys();
-      assert key in AllKeys();
-      assert key in interp;
-    }
-
-    lemma GrowPreservesI()
-      requires WF()
-      requires AllKeys() != {}
-      ensures Grow().WF()
-      ensures Grow().I() == I()
-    {
-      var interp := I().mapp;
-      GrowPreservesWF();
-      var ginterp := Grow().I().mapp;
-      
-      forall key | key in interp
-        ensures key in ginterp && ginterp[key] == interp[key]
-      {
-        Grow().InterpretationDelegation(key);
-      }
-    }
-
     // Insert 
     function InsertLeaf(key: Key, msg: Message) : (result: Node)
     requires Leaf?
     requires WF()
-    ensures result.Leaf?
     ensures result.WF()
+    ensures result.Height() == Height()
+    ensures result.AllKeys() == AllKeys() + {key}
     {
       var llte := Keys.LargestLte(keys, key);
-      if 0 <= llte && keys[llte] == key then
-        Leaf(keys, msgs[llte := msg])
-      else
-        Keys.strictlySortedInsert(keys, key, llte);
-        // TODO: ensures from this lemma can't be asserted?
-        Leaf(insert(keys, key, llte+1), insert(msgs, msg, llte+1))
-    }
-
-    lemma {:timeLimitMultiplier 2} InsertLeafIsCorrect(key: Key, msg: Message)
-    requires Leaf?
-    requires WF()
-    ensures InsertLeaf(key, msg).I() == Buffer(I().mapp[key := msg])
-    ensures InsertLeaf(key, msg).AllKeys() == AllKeys() + {key}
-    {
-      var result := InsertLeaf(key, msg);
-      var llte := Keys.LargestLte(keys, key);
-      if 0 <= llte && keys[llte] == key {
-        assert result.I() == Buffer(I().mapp[key := msg]);
-      } else {
-        Keys.reveal_IsStrictlySorted();
-        forall k | k in result.I().mapp.Keys
-          ensures k in I().mapp.Keys + {key}
-        {
-          var kpos := IndexOf(result.keys, k);
-          if llte + 1 < kpos {
-            assert k == keys[kpos-1];
+      var result := 
+        if 0 <= llte && keys[llte] == key  then 
+          Leaf(keys, msgs[llte := msg])
+        else (
+          assert Keys.IsStrictlySorted(insert(keys, key, llte+1)) by {
+            reveal_insert();
+            Keys.reveal_IsStrictlySorted();
           }
-        }
-        forall k | k in result.AllKeys()
-          ensures k in AllKeys() + {key}
-        {
-          var i :| 0 <= i < |result.keys| && result.keys[i] == k;
-          if i < llte+1 {
-          } else if i == llte+1 {
-          } else {
-            assert k == keys[i-1];
+          Leaf(insert(keys, key, llte+1), insert(msgs, msg, llte+1))
+        );
+
+      assert result.Height() == Height() by { reveal_Height(); }
+      assert result.AllKeys() == AllKeys() + {key} by {
+        if !(0 <= llte && keys[llte] == key) {
+          forall k | k in result.AllKeys()
+            ensures k in AllKeys() + {key}
+          {
+            var i :| 0 <= i < |result.keys| && result.keys[i] == k;
+            if i < llte+1 {
+            } else if i == llte+1 {
+            } else {
+              assert k == keys[i-1];
+            }
           }
         }
       }
+  
+      result   
+    }
+
+    function InsertIndex(key: Key, msg: Message) : (result: Node)
+      requires Index?
+      requires WF()
+      ensures result.Index?
+      ensures result.WF()
+      ensures result.Height() == Height()
+      ensures result.AllKeys() == AllKeys() + {key}
+      decreases Height(), 1
+    {
+      var r := Route(key)+1;
+      ChildrenAreShorter(r);
+      var newChild := children[r].Insert(key, msg);
+      var result := Index(pivots, children[r := newChild]);
+
+      assert result.AllKeys() == AllKeys() + {key} by {
+        var indexKeys := (set i, k | 0 <= i < |children| && k in children[i].AllKeys() :: k);
+        var indexKeys' := (set i, k | 0 <= i < |result.children| && k in result.children[i].AllKeys() :: k);
+
+        forall k 
+          ensures k in indexKeys + {key} <==> k in indexKeys'
+        {
+          if k == key {
+            assert k in result.children[r].AllKeys();
+          } else if k in indexKeys {
+            var i :| 0 <= i < |children| && k in children[i].AllKeys();
+            assert k in result.children[i].AllKeys();
+          } else if k in indexKeys' {
+            var i :| 0 <= i < |result.children| && k in result.children[i].AllKeys();
+            assert k in children[i].AllKeys();
+          }
+        }
+      }
+
+      assert result.WF() by {
+        forall i | 0 <= i < |result.children|-1 
+          ensures result.AllKeysBelowBound(i)
+        {
+          if i == r {
+            forall key' | key' in newChild.AllKeys()
+              ensures Keys.lt(key', pivots[i])
+            {
+              if key' != key {
+                assert AllKeysBelowBound(i);
+              }
+            }
+          } else {
+            assert AllKeysBelowBound(i);
+          }
+        }
+
+        forall i | 0 < i < |result.children|
+          ensures result.AllKeysAboveBound(i)
+        {
+          if i == r {
+            forall key' | key' in newChild.AllKeys()
+              ensures Keys.lte(pivots[i-1], key')
+            {
+              if key' != key {
+                assert AllKeysAboveBound(i);
+              }
+            }
+          } else {
+            assert AllKeysAboveBound(i);
+          }
+        }
+      }
+
+      assert result.Height() == Height() by {
+        assert result.IndexHeights() == IndexHeights(); // trigger
+        reveal_Height();
+      }
+      result
+    }
+
+    function Insert(key: Key, msg: Message) : (result: Node)
+      requires WF()
+      ensures result.WF()
+      ensures result.Height() == Height()
+      ensures result.AllKeys() == AllKeys() + {key}
+      decreases Height(), 2
+    {
+      if Leaf? 
+      then (
+        InsertLeaf(key, msg)
+      ) else (
+        InsertIndex(key, msg)
+      )
     }
 
     // Split 
-
     predicate SplitLeaf(leftleaf: Node, rightleaf: Node, pivot: Key)
     {
       && Leaf?
@@ -306,46 +378,12 @@ module PivotBranchMod {
       && Keys.lte(pivot, rightleaf.keys[0])
     }
 
-    lemma SplitLeafPreservesWF(leftleaf: Node, rightleaf: Node, pivot: Key)
-      requires WF()
-      requires SplitLeaf(leftleaf, rightleaf, pivot)
-      ensures leftleaf.WF()
-      ensures rightleaf.WF()
-    {
-      Keys.StrictlySortedSubsequence(keys, 0, |leftleaf.keys|);
-      Keys.StrictlySortedSubsequence(keys, |leftleaf.keys|, |keys|);
-      assert Keys.IsStrictlySorted(keys[|leftleaf.keys|..|keys|]);
-      assert rightleaf.keys == keys[|leftleaf.keys|..|keys|];
-    }
-
     function SubIndex(from: int, to: int) : (result : Node)
     requires Index?
     requires |children| == |pivots| + 1
     requires 0 <= from < to <= |children|
     {
       Index(pivots[from..to-1], children[from..to])
-    }
-
-    lemma SubIndexPreservesWF(from: int, to: int)
-      requires WF()
-      requires Index?
-      requires 0 <= from < to <= |children|
-      ensures SubIndex(from, to).WF()
-    {
-      Keys.StrictlySortedSubsequence(pivots, from, to-1);
-      var subindex := SubIndex(from, to);
-      forall i | 0 <= i < to - from - 1
-        ensures subindex.AllKeysBelowBound(i)
-      {
-        assert AllKeysBelowBound(from + i);
-      }
-      forall i | 0 < i < to - from
-        ensures subindex.AllKeysAboveBound(i)
-      {
-        assert AllKeysAboveBound(from + i);
-      }
-      assert |subindex.pivots| == |subindex.children| - 1;
-      assert subindex.WF();
     }
 
     predicate SplitIndex(leftindex: Node, rightindex: Node, pivot: Key)
@@ -363,22 +401,134 @@ module PivotBranchMod {
       && pivot == pivots[|leftindex.pivots|]
     }
 
-    lemma SplitIndexPreservesWF(leftindex: Node, rightindex: Node, pivot: Key)
-      requires WF()
-      requires SplitIndex(leftindex, rightindex, pivot)
-      ensures leftindex.WF()
-      ensures rightindex.WF()
-    {
-      SubIndexPreservesWF(0, |leftindex.children|);
-      SubIndexPreservesWF(|leftindex.children|, |children|);
-    }
-
     predicate SplitNode(leftnode: Node, rightnode: Node, pivot: Key)
     {
       || SplitLeaf(leftnode, rightnode, pivot)
       || SplitIndex(leftnode, rightnode, pivot)
     }
 
-    // TODO: add in SplitIndexInterpretation, SplitNodeInterpretation
+    predicate SplitChildOfIndex(newIndex: Node, pivot: Key, childIdx: nat)
+    {
+      && Index?
+      && newIndex.Index?
+      && 0 <= childIdx < |children|
+      && |children| == |pivots| + 1
+      && |newIndex.children| == |children| + 1
+      && newIndex.pivots == insert(pivots, pivot, childIdx)
+      && newIndex.children == replace1with2(children, newIndex.children[childIdx], newIndex.children[childIdx+1], childIdx)
+      && children[childIdx].SplitNode(newIndex.children[childIdx], newIndex.children[childIdx+1], pivot)
+    }
+  }
+
+  // path 
+  datatype Path = Path(node: Node, key: Key, depth: nat)
+  {
+    function Subpath() : (out: Path)
+      requires 0 < depth
+      requires node.WF()
+      requires node.Index?
+    {
+      Path(node.children[node.Route(key)+1], key, depth-1)
+    }
+
+    predicate Valid()
+      decreases depth
+    {
+      && node.WF()
+      && (0 < depth ==> node.Index?)
+      && (0 < depth ==> Subpath().Valid())
+    }
+
+    function Target() : (out: Node)
+      requires Valid()
+      ensures out.WF()
+      decreases depth
+    {
+      if 0 == depth
+      then node
+      else Subpath().Target()
+    }
+  }
+
+  // SM
+  datatype Variables = Variables(root: Node)
+  {
+    predicate WF()
+    {
+      root.WF()
+    }
+  }
+
+  predicate Query(v: Variables, v': Variables, lbl: TransitionLabel)
+  {
+    && lbl.QueryLabel?
+    && v.WF()
+    && v.root.Query(lbl.key) == lbl.msg
+    && v' == v
+  }
+
+  predicate Insert(v: Variables, v': Variables, lbl: TransitionLabel)
+  {
+    && lbl.InsertLabel?
+    && v.WF()
+    && v'.root == v.root.Insert(lbl.key, lbl.msg)
+  }
+
+  predicate Grow(v: Variables, v': Variables, lbl: TransitionLabel)
+  {
+    && lbl.InternalLabel?
+    && v.WF()
+    && v'.root == v.root.Grow()
+  }
+
+  predicate ValidSplit(path: Path, newNode: Node)
+    decreases path.depth
+  {
+    && path.Valid()
+    && var r := path.node.Route(path.key)+1;
+    && (path.depth > 0 ==> 
+      && newNode.Index?
+      && path.node.pivots == newNode.pivots
+      && |path.node.children| == |newNode.children|
+      && (forall i:nat | i < |path.node.children| && i != r
+       :: path.node.children[i] == newNode.children[i])
+      && ValidSplit(path.Subpath(), newNode.children[r]))
+    && (path.depth == 0 ==>
+      && path.node.SplitChildOfIndex(newNode, path.key, r))
+  }
+
+  predicate Split(v: Variables, v': Variables, lbl: TransitionLabel, path: Path)
+  {
+    && lbl.InternalLabel?
+    && v.WF()
+    && path.node == v.root // start from root
+    && ValidSplit(path, v'.root)
+  }
+
+  // public:
+
+  predicate Init(v: Variables)
+  {
+    && v.root == Leaf([], [])
+  }
+
+  datatype Step =
+    | QueryStep()
+    | InsertStep()
+    | GrowStep()
+    | SplitStep(path: Path)
+
+  predicate NextStep(v: Variables, v': Variables, lbl: TransitionLabel, step: Step)
+  {
+    && match step {
+        case QueryStep() => Query(v, v', lbl)
+        case InsertStep() => Insert(v, v', lbl)
+        case GrowStep() => Grow(v, v', lbl)
+        case SplitStep(path) => Split(v, v', lbl, path)
+      }
+  }
+
+  predicate Next(v: Variables, v': Variables, lbl: TransitionLabel) {
+    exists step: Step :: NextStep(v, v', lbl, step)
   }
 }
