Splinter/Betree/PivotBranchRefinement.i.dfy
@@ -1,0 +1,385 @@
+// Copyright 2018-2021 VMware, Inc., Microsoft Inc., Carnegie Mellon University, ETH Zurich, and University of Washington
+// SPDX-License-Identifier: BSD-2-Clause
+ 
+// include "../../lib/Base/KeyType.s.dfy"
+// include "../../Spec/Message.s.dfy"
+// include "../../lib/Base/Option.s.dfy"
+// include "../../lib/Base/Maps.i.dfy"
+// include "../../lib/Base/Sequences.i.dfy"
+// include "../../lib/Base/total_order_impl.i.dfy"
+
+// include "Buffer.i.dfy"
+// include "Domain.i.dfy"
+include "PivotBranch.i.dfy"
+
+module PivotBranchRefinement {
+  import opened Maps
+  import opened Options
+  import opened KeyType
+  import opened ValueMessage
+  import opened Sequences
+  import opened DomainMod
+  import opened BufferMod
+  import opened PivotBranchMod
+  import KeysImpl = Lexicographic_Byte_Order_Impl
+  import Keys = KeysImpl.Ord
+
+  // a data structure refinement: pivot branch => buffer
+
+  lemma GrowPreservesWF(node: Node)
+    requires node.WF()
+    requires node.AllKeys() != {}
+    ensures node.Grow().WF()
+  {
+    assert Keys.IsStrictlySorted([]) by {
+      Keys.reveal_IsStrictlySorted();
+    }
+  }
+
+  lemma GrowPreservesAllKeys(node: Node)
+    requires node.WF()
+    ensures node.Grow().AllKeys() == node.AllKeys()
+  {
+    assert forall key :: key in node.AllKeys() ==> key in node.Grow().children[0].AllKeys();
+  }
+
+  lemma InterpretationDelegation(node: Node, key: Key)
+    requires node.WF()
+    requires node.Index?
+    requires key in node.children[Keys.LargestLte(node.pivots, key)+1].I().mapp
+    ensures MapsTo(node.I().mapp, key, node.children[Keys.LargestLte(node.pivots, key)+1].I().mapp[key])
+  {
+    var interp := node.I().mapp;
+    assert key in node.children[Keys.LargestLte(node.pivots, key)+1].AllKeys();
+    assert key in node.AllKeys();
+    assert key in interp;
+  }
+
+  // lemma AllKeysIsConsistentWithInterpretation(node: Node, key: Key)
+  //   requires node.WF()
+  //   requires key in node.I().mapp
+  //   ensures key in node.AllKeys()
+  //   ensures node.Index? ==> 
+  //     node.WF() && key in node.AllKeys(node.children[Keys.LargestLte(node.pivots, key) + 1])
+  // {
+  //   if node.Index? {
+  //     assert key in (node.children[Keys.LargestLte(node.pivots, key) + 1]);
+  //   }
+  // }
+
+  lemma GrowPreservesI(node: Node)
+    requires node.WF()
+    requires node.AllKeys() != {}
+    ensures node.Grow().WF()
+    ensures node.Grow().I() == node.I()
+  {
+    var interp := node.I().mapp;
+    GrowPreservesWF(node);
+    var ginterp := node.Grow().I().mapp;
+      
+    forall key | key in interp
+      ensures key in ginterp && ginterp[key] == interp[key]
+    {
+      InterpretationDelegation(node.Grow(), key);
+    }
+  }
+
+  lemma {:timeLimitMultiplier 2} InsertLeafIsCorrect(node: Node, key: Key, msg: Message)
+    requires node.Leaf?
+    requires node.WF()
+    ensures node.InsertLeaf(key, msg).I() == Buffer(node.I().mapp[key := msg])
+    // ensures node.InsertLeaf(key, msg).AllKeys() == node.AllKeys() + {key}
+  {
+    var result := node.InsertLeaf(key, msg);
+    var llte := Keys.LargestLte(node.keys, key);
+    if 0 <= llte && node.keys[llte] == key {
+      assert result.I() == Buffer(node.I().mapp[key := msg]);
+    } else {
+      Keys.reveal_IsStrictlySorted();
+      forall k | k in result.I().mapp.Keys
+        ensures k in node.I().mapp.Keys + {key}
+      {
+        var kpos := IndexOf(result.keys, k);
+        if llte + 1 < kpos {
+          assert k == node.keys[kpos-1];
+        }
+      }
+      // forall k | k in result.AllKeys()
+      //   ensures k in node.AllKeys() + {key}
+      // {
+      //   var i :| 0 <= i < |result.keys| && result.keys[i] == k;
+      //   if i < llte+1 {
+      //   } else if i == llte+1 {
+      //   } else {
+      //     assert k == node.keys[i-1];
+      //   }
+      // }
+    }
+  }
+
+  lemma SplitLeafPreservesWF(node: Node, leftleaf: Node, rightleaf: Node, pivot: Key)
+    requires node.WF()
+    requires node.SplitLeaf(leftleaf, rightleaf, pivot)
+    ensures leftleaf.WF()
+    ensures rightleaf.WF()
+  {
+    Keys.StrictlySortedSubsequence(node.keys, 0, |leftleaf.keys|);
+    Keys.StrictlySortedSubsequence(node.keys, |leftleaf.keys|, |node.keys|);
+    assert Keys.IsStrictlySorted(node.keys[|leftleaf.keys|..|node.keys|]);
+    assert rightleaf.keys == node.keys[|leftleaf.keys|..|node.keys|];
+  }
+
+  lemma SubIndexPreservesWF(node: Node, from: int, to: int)
+    requires node.WF()
+    requires node.Index?
+    requires 0 <= from < to <= |node.children|
+    ensures node.SubIndex(from, to).WF()
+  {
+    Keys.StrictlySortedSubsequence(node.pivots, from, to-1);
+    var subindex := node.SubIndex(from, to);
+    forall i | 0 <= i < to - from - 1
+      ensures subindex.AllKeysBelowBound(i)
+    {
+      assert node.AllKeysBelowBound(from + i);
+    }
+    forall i | 0 < i < to - from
+      ensures subindex.AllKeysAboveBound(i)
+    {
+      assert node.AllKeysAboveBound(from + i);
+    }
+    assert |subindex.pivots| == |subindex.children| - 1;
+    assert subindex.WF();
+  }
+
+  lemma SplitIndexPreservesWF(node: Node, leftindex: Node, rightindex: Node, pivot: Key)
+    requires node.WF()
+    requires node.SplitIndex(leftindex, rightindex, pivot)
+    ensures leftindex.WF()
+    ensures rightindex.WF()
+  {
+    SubIndexPreservesWF(node, 0, |leftindex.children|);
+    SubIndexPreservesWF(node, |leftindex.children|, |node.children|);
+  }
+
+  lemma SplitNodePreservesWF(node: Node, leftnode: Node, rightnode: Node, pivot: Key)
+    requires node.SplitNode(leftnode, rightnode, pivot)
+    requires node.WF()
+    ensures leftnode.WF()
+    ensures rightnode.WF()
+  {
+    if node.SplitLeaf(leftnode, rightnode, pivot) {
+      SplitLeafPreservesWF(node, leftnode, rightnode, pivot);
+    } else {
+      SplitIndexPreservesWF(node, leftnode, rightnode, pivot);
+    }
+  }
+
+  lemma {:timeLimitMultiplier 4} SplitLeafInterpretation(oldleaf: Node, leftleaf: Node, rightleaf: Node, pivot: Key)
+    requires oldleaf.SplitLeaf(leftleaf, rightleaf, pivot)
+    requires oldleaf.WF()
+    requires leftleaf.WF()
+    requires rightleaf.WF()
+    ensures oldleaf.I().mapp == Keys.MapPivotedUnion(leftleaf.I().mapp, pivot, rightleaf.I().mapp)
+  {
+    var oldint := oldleaf.I().mapp;
+    var leftint := leftleaf.I().mapp;
+    var rightint := rightleaf.I().mapp;
+    var newint := Keys.MapPivotedUnion(leftint, pivot, rightint);
+
+    forall key | key in oldint
+      ensures key in newint && newint[key] == oldint[key]
+    {
+      var llte := Keys.LargestLte(oldleaf.keys, key);
+      Keys.lteTransitiveForall();
+
+      if llte < |leftleaf.keys| {
+        Keys.PosEqLargestLte(leftleaf.keys, key, llte);
+        Keys.IsStrictlySortedImpliesLt(oldleaf.keys, llte, |leftleaf.keys|);
+        assert Keys.lt(oldleaf.keys[llte], pivot);
+      } else {
+        var rightllte := llte - |leftleaf.keys|;
+        Keys.PosEqLargestLte(rightleaf.keys, key, rightllte);
+        if |leftleaf.keys| < llte {
+          Keys.IsStrictlySortedImpliesLt(oldleaf.keys, |leftleaf.keys|, llte);
+        }
+      }
+    }
+
+    forall key | key in newint
+      ensures key in oldint && oldint[key] == newint[key]
+    {
+      if Keys.lt(key, pivot) {
+        var llte := Keys.LargestLte(leftleaf.keys, key);
+        Keys.PosEqLargestLte(oldleaf.keys, key, llte);
+      } else {
+        var llte := Keys.LargestLte(rightleaf.keys, key);
+        Keys.PosEqLargestLte(oldleaf.keys, key, |leftleaf.keys| + llte);
+      }
+    }
+  }
+
+  lemma SplitIndexInterpretation1(oldindex: Node, leftindex: Node, rightindex: Node, pivot: Key)
+    requires oldindex.WF()
+    requires leftindex.WF()
+    requires rightindex.WF()
+    requires oldindex.SplitIndex(leftindex, rightindex, pivot)
+    ensures forall key :: key in oldindex.I().mapp ==>
+      MapsTo(Keys.MapPivotedUnion(leftindex.I().mapp, pivot, rightindex.I().mapp), 
+        key, oldindex.I().mapp[key])
+  {
+    var oldint := oldindex.I().mapp;
+    var leftint := leftindex.I().mapp;
+    var rightint := rightindex.I().mapp;
+    var newint := Keys.MapPivotedUnion(leftint, pivot, rightint);
+
+    forall key | key in oldint
+      ensures MapsTo(newint, key, oldint[key])
+    {
+      var llte := Keys.LargestLte(oldindex.pivots, key);
+
+      if Keys.lt(key, pivot) { 
+        Keys.LargestLteSubsequence(oldindex.pivots, key, 0, |leftindex.pivots|);
+        assert leftindex.children[llte+1] == oldindex.children[llte+1];
+        InterpretationDelegation(leftindex, key);
+      } else {
+        Keys.LargestLteSubsequence(oldindex.pivots, key, |leftindex.pivots|+1, |oldindex.pivots|);
+        assert rightindex.children[llte - |leftindex.children| + 1] == oldindex.children[llte + 1];
+        InterpretationDelegation(rightindex, key);
+      }
+    }
+  }
+  
+  lemma SplitIndexInterpretation2(oldindex: Node, leftindex: Node, rightindex: Node, pivot: Key)
+    requires oldindex.WF()
+    requires leftindex.WF()
+    requires rightindex.WF()
+    requires oldindex.SplitIndex(leftindex, rightindex, pivot)
+    ensures oldindex.I().mapp.Keys >=
+            Keys.MapPivotedUnion(leftindex.I().mapp, pivot, rightindex.I().mapp).Keys
+  {
+    var oldint := oldindex.I().mapp;
+    var leftint := leftindex.I().mapp;
+    var rightint := rightindex.I().mapp;
+    var newint := Keys.MapPivotedUnion(leftint, pivot, rightint);
+
+    forall key | key in newint
+      ensures key in oldint
+    {
+      if Keys.lt(key, pivot) {
+        Keys.LargestLteSubsequence(oldindex.pivots, key, 0, |leftindex.pivots|);
+      } else {
+        Keys.LargestLteSubsequence(oldindex.pivots, key, |leftindex.pivots|+1, |oldindex.pivots|);
+      }
+      InterpretationDelegation(oldindex, key);
+    }
+  }
+
+  lemma SplitIndexInterpretation(oldindex: Node, leftindex: Node, rightindex: Node, pivot: Key)
+    requires oldindex.WF()
+    requires leftindex.WF()
+    requires rightindex.WF()
+    requires oldindex.SplitIndex(leftindex, rightindex, pivot)
+    ensures oldindex.I().mapp ==
+            Keys.MapPivotedUnion(leftindex.I().mapp, pivot, rightindex.I().mapp)
+  {
+    SplitIndexInterpretation1(oldindex, leftindex, rightindex, pivot);
+    SplitIndexInterpretation2(oldindex, leftindex, rightindex, pivot);
+  }
+
+  lemma SplitNodeInterpretation(oldnode: Node, leftnode: Node, rightnode: Node, pivot: Key)
+    requires oldnode.WF()
+    requires leftnode.WF()
+    requires rightnode.WF()
+    requires oldnode.SplitNode(leftnode, rightnode, pivot)
+    ensures oldnode.I().mapp == Keys.MapPivotedUnion(leftnode.I().mapp, pivot, rightnode.I().mapp) 
+  {
+    if oldnode.SplitLeaf(leftnode, rightnode, pivot) {
+      SplitLeafInterpretation(oldnode, leftnode, rightnode, pivot);
+    } else {
+      SplitIndexInterpretation(oldnode, leftnode, rightnode, pivot);
+    }
+  }
+
+   lemma SplitLeafAllKeys(oldnode: Node, leftnode: Node, rightnode: Node, pivot: Key)
+    requires oldnode.WF()
+    requires leftnode.WF()
+    requires rightnode.WF()
+    requires oldnode.SplitLeaf(leftnode, rightnode, pivot)
+    ensures oldnode.AllKeys() == leftnode.AllKeys() + rightnode.AllKeys()
+    ensures forall key :: key in leftnode.AllKeys() <==> (Keys.lt(key, pivot) && key in oldnode.AllKeys())
+    ensures forall key :: key in rightnode.AllKeys() <==> (Keys.lte(pivot, key) && key in oldnode.AllKeys())
+  {
+    Keys.transitivity_forall();
+
+    forall key | key in leftnode.AllKeys()
+      ensures Keys.lt(key, pivot)
+    {
+      var i :| 0 <= i < |leftnode.keys| && key == leftnode.keys[i];
+      Keys.IsStrictlySortedImpliesLte(oldnode.keys, i, |leftnode.keys|-1);
+    }
+    forall key | key in rightnode.AllKeys()
+      ensures Keys.lte(pivot, key)
+    {
+      var i :| 0 <= i < |rightnode.keys| && key == rightnode.keys[i];
+      Keys.IsSortedImpliesLte(oldnode.keys, |leftnode.keys|, |leftnode.keys| + i);
+    }
+  }
+
+  lemma SplitIndexAllKeys(oldnode: Node, leftnode: Node, rightnode: Node, pivot: Key)
+    requires oldnode.WF()
+    requires leftnode.WF()
+    requires rightnode.WF()
+    requires oldnode.SplitIndex(leftnode, rightnode, pivot)
+    ensures oldnode.AllKeys() == leftnode.AllKeys() + rightnode.AllKeys() + {pivot}
+    ensures forall key :: key in leftnode.AllKeys() <==> (Keys.lt(key, pivot) && key in oldnode.AllKeys())
+    ensures forall key :: key in (rightnode.AllKeys() + {pivot}) <==> (Keys.lte(pivot, key) && key in oldnode.AllKeys())
+  {
+    Keys.transitivity_forall();
+
+    forall key | key in leftnode.AllKeys()
+      ensures Keys.lt(key, pivot)
+    {
+      if i :| 0 <= i < |leftnode.pivots| && key == leftnode.pivots[i] {
+        Keys.IsStrictlySortedImpliesLt(oldnode.pivots, i, |leftnode.pivots|);
+      } else {
+        var i :| 0 <= i < |leftnode.children| && key in leftnode.children[i].AllKeys();
+        assert oldnode.AllKeysBelowBound(i);
+        if i < |leftnode.pivots| {
+          Keys.IsStrictlySortedImpliesLt(oldnode.pivots, i, |leftnode.pivots|);
+        }
+      }
+    }
+
+    forall key | key in rightnode.AllKeys()
+      ensures Keys.lte(pivot, key)
+    {
+      if i :| 0 <= i < |rightnode.pivots| && key == rightnode.pivots[i] {
+        Keys.IsSortedImpliesLte(oldnode.pivots, |leftnode.pivots|, |leftnode.children| + i);
+      } else {
+        var i :| 0 <= i < |rightnode.children| && key in rightnode.children[i].AllKeys();
+        assert oldnode.AllKeysAboveBound(|leftnode.children| + i);
+        Keys.IsSortedImpliesLte(oldnode.pivots, |leftnode.pivots|, |leftnode.children| + i - 1);
+      }
+    }
+    assert Last(rightnode.children) == Last(oldnode.children);
+  }
+
+  lemma SplitNodeAllKeys(oldnode: Node, leftnode: Node, rightnode: Node, pivot: Key)
+    requires oldnode.WF()
+    requires leftnode.WF()
+    requires rightnode.WF()
+    requires oldnode.SplitNode(leftnode, rightnode, pivot)
+    ensures oldnode.AllKeys() <= leftnode.AllKeys() + rightnode.AllKeys() + {pivot}
+    ensures leftnode.AllKeys() + rightnode.AllKeys() <= oldnode.AllKeys()
+    ensures forall key :: key in leftnode.AllKeys() <==> (Keys.lt(key, pivot) && key in oldnode.AllKeys())
+    ensures forall key :: key in (rightnode.AllKeys()) ==> (Keys.lte(pivot, key) && key in oldnode.AllKeys())
+    ensures forall key :: key in (rightnode.AllKeys() + {pivot}) <== (Keys.lte(pivot, key) && key in oldnode.AllKeys())
+  {
+    if oldnode.SplitLeaf(leftnode, rightnode, pivot) {
+      SplitLeafAllKeys(oldnode, leftnode, rightnode, pivot);
+    } else {
+      SplitIndexAllKeys(oldnode, leftnode, rightnode, pivot);
+    }
+  }
+
+}
